boot-strap-pass-2.lisp
@@ -524,6 +524,121 @@
 (defattach (too-many-ifs-pre-rewrite too-many-ifs-pre-rewrite-builtin))
 
 ;;;;;;;;;;;;;;;;;;;;;;;;;;;;;;
+;;; Attachment: ancestors-check
+;;;;;;;;;;;;;;;;;;;;;;;;;;;;;;
+
+(verify-termination-boot-strap pseudo-variantp)
+
+(verify-termination-boot-strap member-char-stringp)
+
+(verify-termination-boot-strap terminal-substringp1)
+
+(verify-termination-boot-strap terminal-substringp)
+
+(verify-termination-boot-strap evg-occur)
+
+(verify-termination-boot-strap min-fixnum)
+
+(verify-termination-boot-strap fn-count-evg-rec) ; but not guards
+
+(defthm fn-count-evg-rec-type-prescription
+  (implies (natp acc)
+           (natp (fn-count-evg-rec evg acc calls)))
+  :rule-classes :type-prescription)
+
+(defthm fn-count-evg-rec-bound
+  (< (fn-count-evg-rec evg acc calls)
+     536870912) ; (expt 2 29)
+  :rule-classes :linear)
+
+(verify-guards fn-count-evg-rec)
+
+(verify-termination-boot-strap occur)
+
+(verify-termination-boot-strap worse-than)
+
+(verify-termination-boot-strap worse-than-or-equal)
+
+(verify-termination-boot-strap ancestor-listp)
+
+(verify-termination-boot-strap earlier-ancestor-biggerp)
+
+(verify-termination-boot-strap fn-count-1) ; but not guards
+
+(defthm fn-count-1-type
+  (implies (and (integerp fn-count-acc)
+                (integerp p-fn-count-acc))
+           (and (integerp (car (fn-count-1 flag term 
+                                           fn-count-acc p-fn-count-acc)))
+                (integerp (mv-nth 1 (fn-count-1 flag term 
+                                                fn-count-acc
+                                                p-fn-count-acc)))))
+  :rule-classes ((:forward-chaining
+                  :trigger-terms
+                  ((fn-count-1 flag term fn-count-acc p-fn-count-acc)))))
+
+(verify-guards fn-count-1)
+
+(verify-termination-boot-strap ancestors-check1)
+
+(verify-termination-boot-strap ancestors-check-builtin)
+
+(encapsulate
+ ()
+
+ (local
+  (defthm ancestors-check1-property
+    (mv-let (on-ancestors assumed-true)
+            (ancestors-check1 lit-atm lit fn-cnt p-fn-cnt ancestors tokens)
+            (implies (and on-ancestors
+                          assumed-true)
+                     (member-equal lit (strip-cars ancestors))))
+    :rule-classes nil))
+
+ (defthmd ancestors-check-builtin-property
+   (mv-let (on-ancestors assumed-true)
+           (ancestors-check-builtin lit ancestors tokens)
+           (implies (and on-ancestors
+                         assumed-true)
+                    (member-equal lit (strip-cars ancestors))))
+   :hints (("Goal"
+            :use
+            ((:instance ancestors-check1-property
+                        (lit-atm lit)
+                        (fn-cnt 0)
+                        (p-fn-cnt 0))
+             (:instance ancestors-check1-property
+                        (lit-atm lit)
+                        (fn-cnt (car (fn-count-1 nil lit 0 0)))
+                        (p-fn-cnt (mv-nth 1 (fn-count-1 nil lit 0 0))))
+             (:instance ancestors-check1-property
+                        (lit-atm (cadr lit))
+                        (fn-cnt (car (fn-count-1 nil (cadr lit) 0 0)))
+                        (p-fn-cnt (mv-nth 1
+                                          (fn-count-1 nil (cadr lit) 0
+                                                      0)))))))))
+
+(encapsulate
+ ((ancestors-check (lit ancestors tokens) (mv t t)
+                   :guard (and (pseudo-termp lit)
+                               (ancestor-listp ancestors)
+                               (true-listp tokens))))
+
+ (local (defun ancestors-check (lit ancestors tokens)
+          (ancestors-check-builtin lit ancestors tokens)))
+
+ (defthmd ancestors-check-constraint
+   (mv-let (on-ancestors assumed-true)
+           (ancestors-check lit ancestors tokens)
+           (implies (and on-ancestors
+                         assumed-true)
+                    (member-equal lit (strip-cars ancestors))))
+   :hints (("Goal" :use ancestors-check-builtin-property))))
+
+(defattach (ancestors-check ancestors-check-builtin)
+  :hints (("Goal" :by ancestors-check-builtin-property)))
+
+;;;;;;;;;;;;;;;;;;;;;;;;;;;;;;
 ;;; End
 ;;;;;;;;;;;;;;;;;;;;;;;;;;;;;;
 
